Split compiler in two files
Signed-off-by: Nicolas Iooss <nicolas.iooss_git@polytechnique.org>

compiler.v
@@ -55,42 +55,7 @@ Definition closed_code (n: nat) (c: krivine_code): Prop :=
    exists t: lterm, tau_code c = Some t /\ fr_below n t
 .
 
-(** Correct environment/stack/state (that's the same object) *)
-Inductive correct_env: krivine_env -> Prop :=
-  | Correct_env_nil: correct_env KEnv_nil
-  | Correct_env:
-    forall (c0: krivine_code) (e0 e: krivine_env),
-    closed_code (klength e0) c0 -> correct_env e0 -> correct_env e ->
-    correct_env (KEnv c0 e0 e)
-.
-
-(** A correct state is a correct non-empty environment *)
-Definition correct_state (st: krivine_env) : Prop :=
-  st <> KEnv_nil /\ correct_env st
-.
-
-(** Proofs *)
-(** 5.2. *)
-Theorem compile_term_tau_ident:
-  forall t: lterm, tau_code (comp t) = Some t.
-Proof.
-  induction t; simpl; trivial.
-  rewrite IHt; trivial.
-  rewrite IHt1; rewrite IHt2; trivial.
-Save.
-
-(** 5.3. *)
-Lemma correct_env_is_state:
-  forall (c0: krivine_code) (e0 e: krivine_env),
-  correct_env (KEnv c0 e0 e) -> correct_state (KEnv c0 e0 e).
-Proof.
-  intros c0 e0 e H.
-  unfold correct_state.
-  apply conj; trivial.
-  intro H0. inversion H0.
-Save.
-
-(** An environment with Nop as code is always incorrect *)
+(** Here are some lemmas using closed_code *)
 Lemma not_closed_Nop:
   forall n: nat, ~ closed_code n Nop.
 Proof.
@@ -102,16 +67,7 @@ Proof.
   intro H0.
   inversion H0.
 Save.
-Lemma incorrect_Nop:
-  forall (e0 e: krivine_env), ~ correct_env (KEnv Nop e0 e).
-Proof.
-  intros e0 e H.
-  inversion H.
-  contradict H3.
-  apply not_closed_Nop.
-Save.
 
-(** A state with Access 0 needs a non-empty environment *)
 Lemma not_closed_Access:
   forall (n: nat) (c: krivine_code), ~ closed_code O (Access n c).
 Proof.
@@ -127,29 +83,3 @@ Proof.
   simpl.
   auto with arith.
 Save.
-
-Lemma incorrect_Access:
-  forall (n: nat) (c: krivine_code) (s: krivine_env),
-  ~ correct_env (KEnv (Access n c) KEnv_nil s).
-Proof.
-  intros n c s H.
-  inversion H.
-  contradict H3; simpl.
-  apply not_closed_Access.
-Save.
-(*
-Theorem step_correctness:
-  forall st: krivine_env, correct_state st -> correct_state (krivine_step st).
-Proof.
-  induction st; trivial.
-  induction k; trivial; intro H.
-
-  (* State: Nop st1 st2 *)
-  inversion H.
-  contradict H1.
-  apply incorrect_Nop.
-
-  (* State: (Access n k) st1 st2 *)
-  inversion H.
-(* Not ended *)
-*)
