compiler_correct.v
@@ -1,0 +1,77 @@
+(** 5. Proof of the compiler, with correct states *)
+Require Import compiler krivine List lterm.
+
+(** Correct environment/stack/state (that's the same object) *)
+Inductive correct_env: krivine_env -> Prop :=
+  | Correct_env_nil: correct_env KEnv_nil
+  | Correct_env:
+    forall (c0: krivine_code) (e0 e: krivine_env),
+    closed_code (klength e0) c0 -> correct_env e0 -> correct_env e ->
+    correct_env (KEnv c0 e0 e)
+.
+
+(** A correct state is a correct non-empty environment *)
+Definition correct_state (st: krivine_env) : Prop :=
+  st <> KEnv_nil /\ correct_env st
+.
+
+(** Proofs *)
+(** 5.2. *)
+Theorem compile_term_tau_ident:
+  forall t: lterm, tau_code (comp t) = Some t.
+Proof.
+  induction t; simpl; trivial.
+  rewrite IHt; trivial.
+  rewrite IHt1; rewrite IHt2; trivial.
+Save.
+
+(** 5.3. *)
+Lemma correct_env_is_state:
+  forall (c0: krivine_code) (e0 e: krivine_env),
+  correct_env (KEnv c0 e0 e) -> correct_state (KEnv c0 e0 e).
+Proof.
+  intros c0 e0 e H.
+  unfold correct_state.
+  apply conj; trivial.
+  intro H0. inversion H0.
+Save.
+
+(** An environment with Nop as code is always incorrect *)
+Lemma incorrect_Nop:
+  forall (e0 e: krivine_env), ~ correct_env (KEnv Nop e0 e).
+Proof.
+  intros e0 e H.
+  inversion H.
+  contradict H3.
+  apply not_closed_Nop.
+Save.
+
+(** A state with Access 0 needs a non-empty environment *)
+
+
+Lemma incorrect_Access:
+  forall (n: nat) (c: krivine_code) (s: krivine_env),
+  ~ correct_env (KEnv (Access n c) KEnv_nil s).
+Proof.
+  intros n c s H.
+  inversion H.
+  contradict H3; simpl.
+  apply not_closed_Access.
+Save.
+(*
+Theorem step_correctness:
+  forall st: krivine_env, correct_state st -> correct_state (krivine_step st).
+Proof.
+  induction st; trivial.
+  induction k; trivial; intro H.
+
+  (* State: Nop st1 st2 *)
+  inversion H.
+  contradict H1.
+  apply incorrect_Nop.
+
+  (* State: (Access n k) st1 st2 *)
+  inversion H.
+(* Not ended *)
+
+*)
